Cslib/Computability/Automata/NA/Total.lean
@@ -16,25 +16,25 @@ public import Cslib.Foundations.Semantics.LTS.Total
 
 namespace Cslib.Automata.NA
 
-open Sum ωSequence Acceptor
+open Option ωSequence Acceptor
 
 variable {Symbol State : Type*}
 
 /-- `NA.totalize` makes the original NA total by replacing its LTS with `LTS.totalize`
 and its starting states with their lifted non-sink versions. -/
-def totalize (na : NA State Symbol) : NA (State ⊕ Unit) Symbol where
+def totalize (na : NA State Symbol) : NA (Option State) Symbol where
   toLTS := na.toLTS.totalize
-  start := inl '' na.start
+  start := some '' na.start
 
 variable {na : NA State Symbol}
 
 /-- In an infinite execution of `NA.totalize`, as long as the NA stays in a non-sink state,
 the execution so far corresponds to a finite execution of the original NA. -/
-theorem totalize_run_mtr {xs : ωSequence Symbol} {ss : ωSequence (State ⊕ Unit)} {n : ℕ}
-    (h : na.totalize.Run xs ss) (hl : (ss n).isLeft) :
-    ∃ s t, na.MTr s (xs.take n) t ∧ s ∈ na.start ∧ ss 0 = inl s ∧ ss n = inl t := by
+theorem totalize_run_mtr {xs : ωSequence Symbol} {ss : ωSequence (Option State)} {n : ℕ}
+    (h : na.totalize.Run xs ss) (hl : (ss n).isSome) :
+    ∃ s t, na.MTr s (xs.take n) t ∧ s ∈ na.start ∧ ss 0 = some s ∧ ss n = some t := by
   obtain ⟨s, _, eq₁⟩ := h.start
-  obtain ⟨t, eq₂⟩ := isLeft_iff.mp hl
+  obtain ⟨t, eq₂⟩ := isSome_iff_exists.mp hl
   use s, t
   refine ⟨?_, by grind⟩
   -- TODO: `grind` does not use congruence relations with `na.totalize.MTr`
@@ -45,7 +45,7 @@ theorem totalize_run_mtr {xs : ωSequence Symbol} {ss : ωSequence (State ⊕ Un
 `NA.totalize`, provided that the alphabet is inbabited. -/
 theorem totalize_mtr_run [Inhabited Symbol] {xl : List Symbol} {s t : State}
     (hs : s ∈ na.start) (hm : na.MTr s xl t) :
-    ∃ xs ss, na.totalize.Run (xl ++ω xs) ss ∧ ss 0 = inl s ∧ ss xl.length = inl t := by
+    ∃ xs ss, na.totalize.Run (xl ++ω xs) ss ∧ ss 0 = some s ∧ ss xl.length = some t := by
   grind [totalize, Run, LTS.Total.extend_omegaExecution <| LTS.totalize.nonsink_mtr_iff.mpr hm]
 
 namespace FinAcc
@@ -53,7 +53,7 @@ namespace FinAcc
 /-- `NA.totalize` and the original NA accept the same language of finite words,
 as long as the accepting states are also lifted in the obvious way. -/
 theorem totalize_language_eq {na : FinAcc State Symbol} :
-    language (FinAcc.mk na.totalize (inl '' na.accept)) = language na := by
+    language (FinAcc.mk na.totalize (some '' na.accept)) = language na := by
   ext xl
   simp +instances [totalize]
 
