Cslib/Computability/Automata/NA/Loop.lean
@@ -167,14 +167,14 @@ namespace FinAcc
 open scoped Computability
 
 /-- `finLoop na` is the loop construction applied to the "totalized" version of `na`. -/
-def finLoop (na : FinAcc State Symbol) : NA (Unit ⊕ (State ⊕ Unit)) Symbol :=
-  FinAcc.loop ⟨na.totalize, inl '' na.accept⟩
+def finLoop (na : FinAcc State Symbol) : NA (Unit ⊕ Option State) Symbol :=
+  FinAcc.loop ⟨na.totalize, some '' na.accept⟩
 
 /-- `finLoop na` is total, assuming that `na` has at least one start state. -/
 instance [h : Nonempty na.start] : na.finLoop.Total where
   total s x := match s with
-    | inl _ => ⟨inr (inr ()), by simpa [finLoop, loop, NA.totalize, LTS.totalize] using h⟩
-    | inr _ => ⟨inr (inr ()), by grind [finLoop, loop, NA.totalize, LTS.totalize]⟩
+    | inl _ => ⟨inr none, by simpa [finLoop, loop, NA.totalize, LTS.totalize] using h⟩
+    | inr _ => ⟨inr none, by grind [finLoop, loop, NA.totalize, LTS.totalize]⟩
 
 /-- `finLoop na` accepts the Kleene star of the language of `na`, assuming that
 the latter is nonempty. -/
